src/drf/PIStep.v
@@ -216,7 +216,7 @@ Proof.
               rewrite IdentMap.gso; eauto.
             }
     }
-    { inv STEPS. des; [done|].
+    { inv STEPS.
       inv STEP; inv STEP0; try done. econs; eauto; ss.
       - apply IdentMap.eq_leibniz. ii.
         setoid_rewrite IdentMap.Properties.F.map_o in TID0.
@@ -240,7 +240,7 @@ Proof.
           rewrite TID in TID1. inv TID1. eauto. }
         econs; eauto. rewrite IdentMap.gso; eauto.
     }
-    { inv STEPS. des; [done|].
+    { inv STEPS.
       inv STEP; inv STEP0; try done. econs; eauto; ss.
       - apply IdentMap.eq_leibniz. ii.
         setoid_rewrite IdentMap.Properties.F.map_o in TID0.
@@ -269,7 +269,7 @@ Proof.
           - eauto. }
         econs; eauto. rewrite IdentMap.gso; eauto.
     }
-    { inv STEPS. des; [done|].
+    { inv STEPS.
       inv STEP; inv STEP0; try done. econs; eauto; ss.
       - apply IdentMap.eq_leibniz. ii.
         setoid_rewrite IdentMap.Properties.F.map_o in TID0.
@@ -326,7 +326,7 @@ Proof.
           hexploit writing_small_step_fulfilled_new; try exact STEPS'; ss; eauto.
           i. inv H. esplits; eauto.
     }
-    { inv STEPS. des; [done|].
+    { inv STEPS.
       inv STEP; inv STEP0; try done. econs; eauto; ss.
       - apply IdentMap.eq_leibniz. ii.
         setoid_rewrite IdentMap.Properties.F.map_o in TID0.
@@ -383,7 +383,7 @@ Proof.
           hexploit writing_small_step_fulfilled_new; try exact STEPS'; ss; eauto.
           i. inv H. esplits; eauto.
     }
-    { inv STEPS. des; [done|].
+    { inv STEPS.
       inv STEP; inv STEP0; try done. econs; eauto; ss.
       - apply IdentMap.eq_leibniz. ii.
         setoid_rewrite IdentMap.Properties.F.map_o in TID0.
@@ -415,7 +415,7 @@ Proof.
           - eauto. }
         econs; eauto. rewrite IdentMap.gso; eauto.
     }
-    { inv STEPS. des; [done|].
+    { inv STEPS.
       inv STEP; inv STEP0; try done. econs; eauto; ss.
       - apply IdentMap.eq_leibniz. ii.
         setoid_rewrite IdentMap.Properties.F.map_o in TID0.
@@ -615,7 +615,7 @@ Proof.
   inv PSTEPS1. inv USTEP. revert STEPS. condtac; cycle 1.
   { i. destruct cST3. esplits; cycle 1.
     - econs 2; eauto. econs; eauto. econs. econs; eauto.
-      + inv STEPS. des; [done|]. destruct pf; ss. inv STEPT. clear PFREE0. econs; eauto.
+      + inv STEPS. destruct pf; ss. inv STEPT. clear PFREE0. econs; eauto.
         destruct pf; eauto. inv STEP0; ss. inv STEP1; ss.
       + rewrite COND. ss.
     - ss.
@@ -631,13 +631,21 @@ Proof.
     - omega.
   }
   inversion A12. inv PI_STEP. inv USTEP.
-  destruct (ThreadEvent.is_promising e0) as [[]|] eqn:E0.
-  { admit. }
   destruct p.
+  destruct (ThreadEvent.is_lower_none e) eqn: NOTLN.
+  { destruct cST3. esplits; eauto.
+     econs; eauto.
+     econs; try apply NEQ.
+     econs; econs; rewrite ?COND; eauto. 
+     inv STEPT. destruct pf; eauto.
+     inv STEP. inv STEP0. ss. by rewrite NOTLN in PF.
+  }
+
   exploit reorder_promise_small_step; try exact STEPT; eauto.
   { inv WF. auto. }
-  { ii. hexploit pi_wf_small_step_is_reading; try exact WF2; eauto. i.
-    hexploit pi_wf_small_step_is_promising; eauto.
+  { ii. destruct (ThreadEvent.is_promising e0) eqn:E0; [by destruct e0|].
+    ii; hexploit pi_wf_small_step_is_reading; try exact WF2; eauto.
+    i. hexploit pi_wf_small_step_is_promising; eauto.
   }
   { apply rtcn_rtc in A23. inv A12.
     exploit pi_step_except_small_step; eauto. i. destruct cST3. ss.
@@ -648,42 +656,61 @@ Proof.
     { eapply small_step_future; eauto. }
     i. eapply promise_consistent_th_small_step; eauto.
   }
-  i. des. unguardH STEP2. des.
-  { destruct cST3. inv STEP2. esplits; cycle 1.
-    - econs 2; eauto. econs; eauto. econs.
-      econs; eauto.
-      + rewrite E0. ss.
+  i. destruct cST3. subst. des.
+  { destruct (ThreadEvent.is_promising e0) eqn:E0; subst.
+    - exploit IH; try exact A23; eauto.
+      { econs; econs; eauto; ii; by destruct e2', e0. }
+      i. des. esplits; try exact STEPS; eauto.
+    - assert (EQ: e2' = e0). 
+      { by destruct e2', e0; inv EVENT. }
+      subst. esplits; [|econs; try exact A23|]; eauto.
+      econs; eauto. econs; econs.
+      + inv STEP. inv STEP0; [by inv STEP|by eauto]. 
+      + rewrite E0. eauto.
+      + eauto.
       + ii. eapply NOWR0; eauto.
-        eapply small_step_is_promised; eauto.
-    - ss.
-    - omega.
+        inv H. econs; eauto. rewrite <- TID0.
+        symmetry; eapply small_step_find; eauto.
   }
-  assert (STEP1': pi_step_evt false tid0 (cS2, cT1) (cS0, c1')).
-  { econs; eauto. econs; eauto.
-    - rewrite E0. ss.
-    - etrans; eauto. inv STEP0. s. rewrite IdentMap.Facts.add_o. condtac; ss.
-      subst. inv STEP; [|by inv STEP0; inv PROMISING]. inv STEP0. ss. inv PROMISING.
-      rewrite TID0. eauto.
-    - ii. eapply NOWR0; eauto.
-      eapply small_step_is_promised; eauto.
+  assert (STEP0': pi_step_except false tidex (cS2, cT1) (cS0,c1')).
+  { econs; eauto. econs; econs.
+    + eauto.
+    + by destruct e2', e0; ss; inv EVENT.
+    + rewrite LANGMATCH0. 
+      inv STEP2. inv STEP; [|by inv STEP0].
+      s. inv STEP0. destruct (Ident.eq_dec tid0 tid).
+      * subst. by rewrite IdentMap.gss, TID0.
+      * rewrite IdentMap.gso; eauto.
+    + ii. eapply NOWR0; eauto.
+      * by destruct e2'; inv WRITE; destruct e0; inv EVENT.
+      * eapply small_step_is_promised; eauto.
   }
   assert (STEP2': pi_step_evt true tid (cS0, c1') (cS0, cT3)).
   { econs. econs; eauto.
     - rewrite PROMISING. ss.
     - destruct (Ident.eq_dec tid0 tid); subst; ss.
-      admit.
-      (* rewrite E0 in *. *)
-      (* inv STEPS. s. rewrite IdentMap.gso; auto. *)
-      (* inv STEPT0. s. rewrite IdentMap.gso; auto. *)
-    - ii. destruct e1'; ss.
+      rewrite <-(small_step_find STEPT0); eauto.
+      rewrite <-LANGMATCH.
+      destruct (ThreadEvent.is_promising e0); subst; eauto.
+      rewrite (small_step_find STEPS); eauto.
+    - ii. by destruct e1'.
   }
+  assert (STEP1': pi_step_evt false tid0 (cS2, cT1) (cS0, c1')).
+  { econs. econs; eauto.
+    - by destruct e2', e0; inv EVENT.
+    - etrans; eauto. destruct (Ident.eq_dec tid tid0). 
+      + subst. inv STEP2. s. rewrite IdentMap.gss. 
+        inv STEP; [by inv STEP0; rewrite TID0|by inv STEP0; inv PROMISING].
+      + rewrite (small_step_find STEP2); eauto.
+    - ii. eapply NOWR0; eauto.
+      + by destruct e2'; inv WRITE; destruct e0; inv EVENT.
+      + eapply small_step_is_promised; eauto.
+  }
+
   exploit IH; try exact STEP2'; eauto.
   { eapply pi_step_future; eauto. }
-  i. des. esplits; cycle 1.
-  - econs; eauto.
-  - ss.
-  - omega.
-Admitted.
+  i. des. esplits; [|econs; try exact STEPS0|]; eauto; omega.
+Qed.
 
 Lemma rtc_pi_step_remove_promises_aux
       tid tidex cST1 cST2 cST3
