build.sh
@@ -3,4 +3,9 @@
 mkdir -p .build
 rsync -avl --delete --exclude '*.vo' --exclude '*.vio' --exclude '*.v.d' --exclude '*.glob' --exclude '.*.aux' lib src Makefile _CoqProject .build
 cd .build
-make -f Makefile build -j
+if [ -z $* ]
+then
+  make -j -f Makefile build
+else
+  make -j -f Makefile $*
+fi
